SystemFD/Metatheory/Canonicity.lean
@@ -111,51 +111,55 @@ theorem cannonical_head :
   Γ ⊢ t : τ ->
   Γ ⊢ τ : ★ ->
   t.neutral_form = .some (h, ts) ->
-  (Γ.is_ctor h ∨ Γ.is_insttype h)
+  (Γ.is_ctor h ∨ Γ.is_insttype h ∨ OpenVarVal Γ h ts)
 := by
-  sorry
--- intro vt tJ τJ tnf;
--- have tshape := Term.neutral_form_law (Eq.symm tnf)
--- rw[<-tshape] at tJ;
--- have hJ := inversion_apply_spine tJ;
--- cases hJ; case _ τ' hJ =>
--- cases hJ; case _ spTy hJ =>
--- cases hJ; case _ hJ h3 =>
--- cases vt;
--- any_goals(solve | cases tnf)
--- case app h_stable tnf' =>
---   rw[tnf] at tnf'; cases tnf';
---   cases hJ; case _ wf gt =>
---   have τ'J := spine_type_is_type τJ spTy
---   have hJ := Judgment.var wf gt;
---   simp at h_stable;
---   generalize fh : Γ d@ h = f at *;
---   cases f;
---   any_goals (solve | cases gt)
---   all_goals (unfold Frame.is_stable_red at h_stable; simp at h_stable)
---   all_goals (clear h_stable; unfold Frame.get_type at gt; simp at gt; cases gt)
---   case _ =>
---     have h := ctx_get_var_type wf fh;
---     have lem1 := kind_shape h rfl
---     have lem2 := type_shape τ'J (by constructor)
---     exfalso; apply Term.is_kind_disjoint_is_type lem1 lem2
---   case _ =>
---     have h := ctx_get_datatype_kind wf fh;
---     have lem1 := kind_shape h rfl
---     have lem2 := type_shape τ'J (by constructor)
---     exfalso; apply Term.is_kind_disjoint_is_type lem1 lem2
---   case _ =>
---     apply Or.inl;
---     simp; rw[fh]; unfold Frame.is_ctor; simp;
---   case _ =>
---     have h := ctx_get_opent_kind wf fh
---     have lem1 := kind_shape h rfl
---     have lem2 := type_shape τ'J (by constructor)
---     exfalso; apply Term.is_kind_disjoint_is_type lem1 lem2
---   case _ =>
---     apply Or.inr;
---     simp; rw[fh]; unfold Frame.is_insttype; simp;
-
+intro vt tJ τJ tnf;
+have tshape := Term.neutral_form_law (Eq.symm tnf)
+rw[<-tshape] at tJ;
+have hJ := inversion_apply_spine tJ;
+cases hJ; case _ τ' hJ =>
+cases hJ; case _ spTy hJ =>
+cases hJ; case _ hJ h3 =>
+cases vt
+any_goals(solve | cases tnf)
+case app h_stable tnf' =>
+  cases h_stable
+  case _ h_stable =>
+   rw[tnf] at tnf'; cases tnf';
+   cases hJ; case _ wf gt =>
+   have τ'J := spine_type_is_type τJ spTy
+   have hJ := Judgment.var wf gt;
+   simp at h_stable;
+   generalize fh : Γ d@ h = f at *;
+   cases f;
+   any_goals (solve | cases gt)
+   all_goals (unfold Frame.is_stable_red at h_stable; simp at h_stable)
+   all_goals (clear h_stable; unfold Frame.get_type at gt; simp at gt; cases gt)
+   case _ =>
+     have h := ctx_get_var_type wf fh;
+     have lem1 := kind_shape h rfl
+     have lem2 := type_shape τ'J (by constructor)
+     exfalso; apply Term.is_kind_disjoint_is_type lem1 lem2
+   case _ =>
+     have h := ctx_get_datatype_kind wf fh;
+     have lem1 := kind_shape h rfl
+     have lem2 := type_shape τ'J (by constructor)
+     exfalso; apply Term.is_kind_disjoint_is_type lem1 lem2
+   case _ =>
+     apply Or.inl;
+     simp; rw[fh]; unfold Frame.is_ctor; simp;
+   case _ =>
+     have h := ctx_get_opent_kind wf fh
+     have lem1 := kind_shape h rfl
+     have lem2 := type_shape τ'J (by constructor)
+     exfalso; apply Term.is_kind_disjoint_is_type lem1 lem2
+   case _ =>
+     apply Or.inr;
+     simp; rw[fh]; unfold Frame.is_insttype; simp;
+  case _ ovv =>
+    rw[tnf] at tnf'; cases tnf'
+    apply Or.inr; apply Or.inr
+    assumption
 
 inductive ArrowLike : (T : Term) -> Prop where
 | arrowt : ArrowLike (A -t> B)
@@ -170,6 +174,7 @@ inductive LambdaLike (Γ : Ctx Term) : (T : Term) -> Prop where
   LambdaLike Γ t1 ->
   LambdaLike Γ t2 ->
   LambdaLike Γ (t1 ⊕ t2)
+| app : OpenVarVal Γ h τs -> LambdaLike Γ ((#h).apply_spine ts)
 
 @[simp]
 abbrev CanonicalLambdaType (Γ : Ctx Term) : (v : JudgmentVariant) -> JudgmentArgs v -> Prop
@@ -185,165 +190,223 @@ theorem canonical_lambda :
   Judgment v Γ idx ->
   CanonicalLambdaType Γ v idx
 := by
-  sorry
--- intro j; induction j <;> simp at *
--- all_goals (intro h1 h2 h3 h4)
--- any_goals try (solve | cases h1; case _ h1 => cases h1)
--- any_goals try (solve | cases h3)
--- case _ Γ n T wf gt ih =>
---   cases h1; case _ n_stable nnf =>
---   simp at nnf; cases nnf; case _ e1 e2 =>
---   subst e1; subst e2;
---   generalize fh : Γ d@ n = f at *;
---   unfold Frame.get_type at gt;
---   cases h4;
---   case _ =>
---     split at gt;
---     any_goals (solve | cases gt)
---     any_goals (solve | unfold Ctx.is_stable_red at n_stable; unfold Frame.is_stable_red at n_stable;
---                        exfalso; rw[fh] at n_stable; simp at n_stable)
---     all_goals (cases gt)
---     case _ =>
---       have lem := classification_lemma h3; simp at lem;
---       cases lem;
---       case _ =>
---         have wfr := @frame_wf_by_index Γ n wf;
---         have h := ctx_get_var_type wf fh;
---         cases h
---       case _ h =>
---         cases h; case _ k h => cases h; case _ _ h => cases h; case _ h => cases h
---     case _ =>
---       have wfr := @frame_wf_by_index Γ n wf;
---       have h := ctx_get_datatype_kind wf fh;
---       cases h;
---     case _ =>
---       apply LambdaLike.ctor; unfold ValidHeadVariable;
---       apply Exists.intro (n, []);
---       apply And.intro; simp; simp; rw[fh]; unfold Frame.is_ctor; simp
---     case _ =>
---       have wfr := @frame_wf_by_index Γ n wf;
---       have h := ctx_get_opent_kind wf fh;
---       cases h;
---     case _ =>
---       apply LambdaLike.insttype; unfold ValidHeadVariable;
---       apply Exists.intro (n, []);
---       apply And.intro; simp; simp; rw[fh]; unfold Frame.is_insttype; simp
---   case _ =>
---     split at gt;
---     any_goals (solve | cases gt)
---     any_goals (solve | unfold Ctx.is_stable_red at n_stable; unfold Frame.is_stable_red at n_stable;
---                        exfalso; rw[fh] at n_stable; simp at n_stable)
---     all_goals (cases gt)
---     case _ =>
---       have lem := classification_lemma h3; simp at lem;
---       cases lem;
---       case _ =>
---         have wfr := @frame_wf_by_index Γ n wf;
---         have h := ctx_get_var_type wf fh;
---         cases h
---       case _ h =>
---         cases h; case _ k h => cases h; case _ _ h => cases h; case _ h => cases h
---     case _ =>
---       have wfr := @frame_wf_by_index Γ n wf;
---       have h := ctx_get_datatype_kind wf fh;
---       cases h;
---     case _ =>
---       apply LambdaLike.ctor; unfold ValidHeadVariable;
---       apply Exists.intro (n, []);
---       apply And.intro; simp; simp; rw[fh]; unfold Frame.is_ctor; simp
---     case _ =>
---       have wfr := @frame_wf_by_index Γ n wf;
---       have h := ctx_get_opent_kind wf fh;
---       cases h;
---     case _ =>
---       apply LambdaLike.insttype; unfold ValidHeadVariable;
---       apply Exists.intro (n, []);
---       apply And.intro; simp; simp; rw[fh]; unfold Frame.is_insttype; simp
+intro j; induction j <;> simp at *
+all_goals (intro h1 h2 h3 h4)
+any_goals try (solve | cases h1; case _ h1 => cases h1)
+any_goals try (solve | cases h3)
+case var Γ n T wf gt ih =>
+  cases h1; case _ n_stable nnf =>
+  simp at nnf; cases nnf; case _ e1 e2 =>
+  subst e1; subst e2;
+  generalize fh : Γ d@ n = f at *;
+  unfold Frame.get_type at gt;
+  cases h4
+  case arrowt =>
+    split at gt;
+    any_goals (solve | cases gt)
+    all_goals (cases gt)
+    case _ =>
+      have lem := classification_lemma h3; simp at lem;
+      cases lem;
+      case _ =>
+        have wfr := @frame_wf_by_index Γ n wf;
+        have h := ctx_get_var_type wf fh;
+        cases h
+      case _ h =>
+        cases h; case _ k h => cases h; case _ _ h => cases h; case _ h => cases h
+    case _ =>
+      unfold Ctx.is_stable_red at n_stable; unfold Frame.is_stable_red at n_stable;
+      rw[fh] at n_stable; simp at n_stable
+      have wfr := @frame_wf_by_index Γ n wf;
+      cases n_stable; case _ n_stable _ =>
+      simp at n_stable; rw[fh] at n_stable;
+      unfold Frame.is_openm at n_stable; simp at n_stable
+    case _ A B _ =>
+      have wfr := @frame_wf_by_index Γ n wf;
+      replace wfr' := frame_wf_type_implies_kind (A -t> B) wfr
+            (by rw[fh]; unfold Frame.get_type; simp)
+            (by apply Or.inr; apply Or.inl; simp; rw[fh]; unfold Frame.is_datatype; simp)
+      apply LambdaLike.ctor; unfold ValidHeadVariable;
+      apply Exists.intro (n, []);
+      apply And.intro; simp; simp; rw[fh]; unfold Frame.is_ctor; simp
+      have lem : (A -t> B).IsType := type_shape h3 (by constructor)
+      exfalso
+      have lem' := uniqueness_of_kinds lem wfr' h3; cases lem'
+    case _ =>
+      constructor
+      unfold ValidHeadVariable; exists (n, [])
+      constructor <;> simp
+      · rw[fh]; unfold Frame.is_ctor; simp
+    case _ =>
+      have wfr := @frame_wf_by_index Γ n wf;
+      have h := ctx_get_opent_kind wf fh;
+      cases h;
+    case _ =>
+      cases n_stable
+      case _ h => simp at h; rw[fh] at h; unfold Frame.is_stable_red at h; simp at h
+      case _ A B _ h =>
+        apply @LambdaLike.app Γ n [] [] h
+    case _ =>
+      apply LambdaLike.insttype; unfold ValidHeadVariable;
+      apply Exists.intro (n, []);
+      apply And.intro; simp; simp; rw[fh]; unfold Frame.is_insttype; simp
+    case _ =>
+      cases n_stable
+      case _ h => simp at h; rw[fh] at h; unfold Frame.is_stable_red at h; simp at h
+      case _ h => unfold OpenVarVal at h; simp at h; rw[fh] at h; unfold Frame.is_openm at h; simp at h;
+  case allt =>
+    split at gt;
+    any_goals (solve | cases gt)
+    all_goals (cases gt)
+    case _ =>
+      have lem := classification_lemma h3; simp at lem;
+      cases lem;
+      case _ =>
+        have wfr := @frame_wf_by_index Γ n wf;
+        have h := ctx_get_var_type wf fh;
+        cases h
+      case _ h =>
+        cases h; case _ k h => cases h; case _ _ h => cases h; case _ h => cases h
+    case _ =>
+      unfold Ctx.is_stable_red at n_stable; unfold Frame.is_stable_red at n_stable;
+      rw[fh] at n_stable; simp at n_stable
+      have wfr := @frame_wf_by_index Γ n wf;
+      cases n_stable; case _ n_stable _ =>
+      simp at n_stable; rw[fh] at n_stable;
+      unfold Frame.is_openm at n_stable; simp at n_stable
+    case _ A B _ =>
+      have wfr := @frame_wf_by_index Γ n wf;
+      replace wfr' := frame_wf_type_implies_kind (∀[A] B) wfr
+            (by rw[fh]; unfold Frame.get_type; simp)
+            (by apply Or.inr; apply Or.inl; simp; rw[fh]; unfold Frame.is_datatype; simp)
+      apply LambdaLike.ctor; unfold ValidHeadVariable;
+      apply Exists.intro (n, []);
+      apply And.intro; simp; simp; rw[fh]; unfold Frame.is_ctor; simp
+      have lem : (∀[A] B).IsType := type_shape h3 (by constructor)
+      exfalso
+      have lem' := uniqueness_of_kinds lem wfr' h3; cases lem'
+    case _ =>
+      constructor
+      unfold ValidHeadVariable; exists (n, [])
+      constructor <;> simp
+      · rw[fh]; unfold Frame.is_ctor; simp
+    case _ =>
+      have wfr := @frame_wf_by_index Γ n wf;
+      have h := ctx_get_opent_kind wf fh;
+      cases h;
+    case _ =>
+      cases n_stable
+      case _ h => simp at h; rw[fh] at h; unfold Frame.is_stable_red at h; simp at h
+      case _ A B _ h =>
+        apply @LambdaLike.app Γ n [] [] h
+    case _ =>
+      apply LambdaLike.insttype; unfold ValidHeadVariable;
+      apply Exists.intro (n, []);
+      apply And.intro; simp; simp; rw[fh]; unfold Frame.is_insttype; simp
+    case _ =>
+      cases n_stable
+      case _ h => simp at h; rw[fh] at h; unfold Frame.is_stable_red at h; simp at h
+      case _ h => unfold OpenVarVal at h; simp at h; rw[fh] at h; unfold Frame.is_openm at h; simp at h;
 
--- case _ Γ f _ _ _ fJ _ _ ih => -- appk bogus case
---   cases h1; case _ n ts n_stable ts' =>
---   simp at ts'; rw [Option.bind_eq_some] at ts';  cases ts'; case _ w fnf =>
---   cases fnf; case _ fnf ts' =>
---   cases ts';
---   have vf : Val Γ f := by constructor; assumption; assumption
---   generalize fh : Γ d@ w.fst = f at *;
---   have lem := classification_lemma fJ; simp at lem; cases lem;
---   case _ h => cases h; case _ k1 k2 =>
---     have lem1 := kind_shape k2 rfl
---     have lem2 := type_shape h3 (by constructor)
---     exfalso; apply Term.is_kind_disjoint_is_type lem1 lem2
---   case _ h =>
---     cases h; case _ w h =>
---     cases h; case _ wk arrk =>
---     cases arrk; cases wk;
 
--- case lam Γ A t B ih1 ih2 => constructor
+case appk Γ f _ _ _ fJ _ _ ih => -- appk bogus case
+  cases h1; case _ n ts n_stable ts' =>
+  simp at ts'; rw [Option.bind_eq_some_iff] at ts';  cases ts'; case _ w fnf =>
+  cases fnf; case _ fnf ts' =>
+  cases ts';
+  have vf : Val Γ f := by
+    constructor
+    · assumption
+    · cases n_stable;
+      case _ => apply Or.inl; assumption
+      case _ h =>
+        apply Or.inr
+        unfold OpenVarVal at h; cases h; case _ h =>
+        unfold OpenVarVal; constructor
+        · assumption
+        · intro T gt;
+          replace h := h T gt
+          simp at h; omega
+  generalize fh : Γ d@ w.fst = f at *;
+  have lem := classification_lemma fJ; simp at lem; cases lem;
+  case _ h => cases h; case _ k1 k2 =>
+    have lem1 := kind_shape k2 rfl
+    have lem2 := type_shape h3 (by constructor)
+    exfalso; apply Term.is_kind_disjoint_is_type lem1 lem2
+  case _ h =>
+    cases h; case _ w h =>
+    cases h; case _ wk arrk =>
+    cases arrk; cases wk;
 
--- case app Γ f A B a B' fJ aJ h0 ih1 ih2 =>
---   cases h1; case _ n ts n_stable h1 =>
---   simp at h1; rw[Option.bind_eq_some] at h1;
---   cases h1;  case _ ts' fnf =>
---   cases fnf; case _ fnf hts =>
---   cases ts'; case _ x sp =>
---   simp at hts; cases hts; case _ e1 e2 =>
---   subst e1; subst e2
---   have h := Val.app x sp fnf n_stable;
---   simp at *;
---   have lem := classification_lemma fJ; simp at lem;
---   cases lem;
---   case _ h => cases h
---   case _ h =>
---     cases h; case _ k h =>
---     cases h; case _ k h =>
---     cases h; case _ aK bK =>
---     have arrK := Judgment.arrow aK bK;
---     have ih := ih1 h fJ arrK (ArrowLike.arrowt); cases ih;
---     case _ h => cases fnf
---     case _ h => cases fnf
---     case _ h =>
---       apply LambdaLike.ctor;
---       unfold ValidHeadVariable;
---       have fanf := @Term.neutral_form_app f a x sp fnf; symm at fanf;
---       apply Exists.intro (x, sp ++ [(.term, a)]);
---       apply And.intro; assumption; simp;
---       unfold ValidHeadVariable at h; simp at h;
---       cases h; case _ h => cases h; case _ fnf' h =>
---       rw [fnf] at fnf'; cases fnf'; case _ h =>
---       cases h; assumption
---     case _ h =>
---       apply LambdaLike.insttype;
---       unfold ValidHeadVariable;
---       have fanf := @Term.neutral_form_app f a x sp fnf; symm at fanf;
---       apply Exists.intro (x, sp ++ [(.term, a)]);
---       apply And.intro; assumption; simp;
---       unfold ValidHeadVariable at h; simp at h;
---       cases h; case _ h => cases h; case _ fnf' h =>
---       rw [fnf] at fnf'; cases fnf'; case _ h =>
---       cases h; assumption
---     case _ => cases fnf
--- case _ ih1 _ =>
---   cases h1;
---   case _ h => cases h
---   case _ => constructor
+case lam Γ A t B ih1 ih2 => constructor
+case lamt ih1 _ =>
+  cases h1
+  case _ h => cases h
+  case _ => constructor
 
--- case _ Γ f A B a B' fJ aJ _ ih1 ih2 =>
---   cases h1; case _ n ts n_stable h1 =>
---   simp at h1; rw[Option.bind_eq_some] at h1;
---   cases h1;  case _ ts' fnf =>
---   cases fnf; case _ fnf hts =>
---   cases ts'; case _ x sp =>
---   simp at hts; cases hts; case _ e1 e2 =>
---   subst e1; subst e2
---   have h := Val.app x sp fnf n_stable;
---   simp at *;
---   have lem := classification_lemma fJ; simp at lem;
---   cases lem;
---   case _ h => cases h
---   case _ h =>
---     cases h; case _ k h =>
---     cases h; case _ k h =>
---     cases h; case _ aK bK =>
---     have arrK := Judgment.allt aK bK;
+case app Γ f A B a B' fJ aJ h0 ih1 ih2 =>
+  cases h1; case _ n ts n_stable h1 =>
+  simp at h1; rw[Option.bind_eq_some_iff] at h1;
+  cases h1;  case _ ts' fnf =>
+  cases fnf; case _ fnf hts =>
+  cases ts'; case _ x sp =>
+  simp at hts; cases hts; case _ e1 e2 =>
+  subst e1; subst e2
+  -- have h := Val.app x sp fnf n_stable;
+  simp at *;
+  have lem := classification_lemma fJ; simp at lem;
+  cases lem;
+  case _ h => cases h
+  case _ h =>
+    cases h; case _ k h =>
+    cases h; case _ k h =>
+    cases h; case _ aK bK =>
+    have arrK := Judgment.arrow aK bK;
+    -- have ih := ih1 h fJ arrK (ArrowLike.arrowt); cases ih;
+    -- case _ h => cases fnf
+    -- case _ h => cases fnf
+    -- case _ h =>
+    --   apply LambdaLike.ctor;
+    --   unfold ValidHeadVariable;
+    --   have fanf := @Term.neutral_form_app f a x sp fnf; symm at fanf;
+    --   apply Exists.intro (x, sp ++ [(.term, a)]);
+    --   apply And.intro; assumption; simp;
+    --   unfold ValidHeadVariable at h; simp at h;
+    --   cases h; case _ h => cases h; case _ fnf' h =>
+    --   rw [fnf] at fnf'; cases fnf'; case _ h =>
+    --   cases h; assumption
+    -- case _ h =>
+    --   apply LambdaLike.insttype;
+    --   unfold ValidHeadVariable;
+    --   have fanf := @Term.neutral_form_app f a x sp fnf; symm at fanf;
+    --   apply Exists.intro (x, sp ++ [(.term, a)]);
+    --   apply And.intro; assumption; simp;
+    --   unfold ValidHeadVariable at h; simp at h;
+    --   cases h; case _ h => cases h; case _ fnf' h =>
+    --   rw [fnf] at fnf'; cases fnf'; case _ h =>
+    --   cases h; assumption
+    -- case _ => cases fnf
+    sorry
+
+case _ Γ f A B a B' fJ aJ _ ih1 ih2 =>
+  cases h1; case _ n ts n_stable h1 =>
+  simp at h1; rw[Option.bind_eq_some_iff] at h1;
+  cases h1;  case _ ts' fnf =>
+  cases fnf; case _ fnf hts =>
+  cases ts'; case _ x sp =>
+  simp at hts; cases hts; case _ e1 e2 =>
+  subst e1; subst e2
+  -- have h := Val.app x sp fnf n_stable;
+  simp at *;
+  have lem := classification_lemma fJ; simp at lem;
+  cases lem;
+  case _ h => cases h
+  case _ h =>
+    cases h; case _ k h =>
+    cases h; case _ k h =>
+    cases h; case _ aK bK =>
+    have arrK := Judgment.allt aK bK;
+    sorry
 --     have ih := ih1 h fJ arrK (ArrowLike.allt); cases ih;
 --     case _ h => cases fnf
 --     case _ h => cases fnf
@@ -375,3 +438,10 @@ theorem canonical_lambda :
 --     replace ih3 := ih3 v1 j3 h3 h4
 --     replace ih4 := ih4 v2 j4 h3 h4
 --     apply LambdaLike.choice ih3 ih4
+case refl   => cases h4
+case choice ih1 ih2 =>
+  cases h2
+  cases h1
+  case _ h1 => simp at h1
+  case _ v1 v2 =>
+    apply LambdaLike.choice <;> simp_all
