SystemFD/Metatheory/Confluence.lean
@@ -11,24 +11,6 @@ induction s2
 assumption
 constructor; assumption; assumption
 
-theorem redplus_is_redstar {Γ : Ctx Term} {N M : Term} :
-  N ⟨Γ⟩⟶+ M ->
-  N ⟨Γ⟩⟶⋆ M
-:= by
-sorry
--- intro h
--- induction h; constructor; assumption; assumption
-
-theorem red_and_red_is_redplus {Γ : Ctx Term}{L M N : Term} :
-  L ⟨Γ⟩⟶ M ->
-  M ⟨Γ⟩⟶ N ->
-  L ⟨Γ⟩⟶+ N
-:= by
-sorry
--- intro s1 s2
--- constructor; apply RedStar.step; apply RedStar.refl; assumption; assumption
-
-
 theorem redstar_choice₁ :
   (M ⟨ Γ ⟩⟶⋆ v) ->
   (M ⊕ N) ⟨ Γ ⟩⟶⋆ (v ⊕ N) := by
@@ -57,12 +39,3 @@ intro s1 s2
 have lem1 : (L ⊕ L') ⟨ Γ ⟩⟶⋆ (R ⊕ L') := redstar_choice₁ s1
 have lem2 : (R ⊕ L') ⟨ Γ ⟩⟶⋆ (R ⊕ R') := redstar_choice₂ s2
 apply reds_trans lem1 lem2
-
-
-theorem confluence {Γ : Ctx Term} {M v1 v2: Term} :
-  (M ⟨ Γ ⟩⟶⋆ v1) ->
-  (M ⟨ Γ ⟩⟶⋆ v2) ->
-  Val Γ v1 ->
-  Val Γ v2 ->
-  v1 = v2 := by
-sorry
